

Solution: All the productions in the grammar are not in CNF. We have to convert them into CNF keeping the language generating power the same. Let us replace 'a' by D_a , 'b' by D_b , and 'c' by D_c . So, three new productions $D_a \rightarrow a$, $D_b \rightarrow b$, and $D_c \rightarrow c$ are added to the grammar. By replacing 'a' by D_a , 'b' by D_b , and 'c' by D_c , and adding three productions, the modified grammar becomes

$$\begin{aligned} S &\rightarrow ABD_a \\ A &\rightarrow DaDaD_b \\ B &\rightarrow AD_c \\ D_a &\rightarrow a \\ D_b &\rightarrow b \\ D_c &\rightarrow c \end{aligned}$$

$S \rightarrow ABD_a$ and $A \rightarrow DaDaD_b$ are not in CNF. Take two non-terminals E and F. Replace AB by E and DaDa by F. So, two new productions $E \rightarrow AB$ and $F \rightarrow DaDa$ will be added to the grammar. By replacement and adding the productions, the modified grammar will be

$$\begin{aligned} S &\rightarrow ABD_a \\ A &\rightarrow DaDaD_b \\ B &\rightarrow AD_c \\ D_a &\rightarrow a \\ D_b &\rightarrow b \\ D_c &\rightarrow c \\ E &\rightarrow AB \\ F &\rightarrow DaDa \end{aligned}$$

In the previous grammar, all the productions are in the form of Non-terminal \rightarrow string of exactly two non-terminals or non-terminal \rightarrow single terminal. So, the grammar is in CNF.

Example 6.39

Convert the following grammar into CNF.

$$\begin{aligned} E &\rightarrow E + E \\ E &\rightarrow E^*E \\ E &\rightarrow id \end{aligned}$$

where $\Sigma = (+, *, id)$

Solution: Except $E \rightarrow id$, all the other productions of the grammar are not in CNF. In the grammar $E \rightarrow E + E$ and $E \rightarrow E^*E$, there are two terminals + and *. Take two non-terminals C and D for replacing + and *, respectively. Two new productions will be added to the grammar. By replacing + and *, the modified production rules will be

$$\begin{aligned} E &\rightarrow ECE \\ E &\rightarrow EDE \\ E &\rightarrow id \\ C &\rightarrow + \\ D &\rightarrow * \end{aligned}$$

In the production rules $E \rightarrow ECE$ and $E \rightarrow EDE$, there are three non-terminals. Replace EC by another non-terminal F and ED by G . So, two new productions $F \rightarrow EC$ and $G \rightarrow ED$ will be added to the grammar. By replacing and adding the new productions, the modified grammar will be